theories/L6_PCPS/inline_proto.v
@@ -15,15 +15,20 @@ Require Import Coq.Structures.OrdersEx.
 Import MonadNotation.
 Open Scope monad_scope. *)
 
-Require Import Coq.ZArith.ZArith.
-Require Import L6.freshen L6.state L6.identifiers L6.shrink_cps L6.cps_proto.
+Require Import Coq.Sets.Ensembles Coq.ZArith.ZArith.
+Require Import L6.Ensembles_util L6.map_util.
+Require Import L6.state L6.alpha_conv L6.identifiers L6.functions L6.shrink_cps.
+Require Import L6.Prototype.
+Require Import L6.cps_proto L6.proto_util.
+
+Require Import Lia.
 
 Require Import Coq.Lists.List.
 Import ListNotations.
 
-Definition r_map : Set := M.tree var.
+(* -------------------- Inlining heuristics --------------------
 
-(* Inlining heuristic. Rather than parameterizing by [St] as in inline.v, the heuristic is
+   Rather than parameterizing by [St] as in inline.v, the heuristic is
    represented as a record of closures (like an OOP class). This is to allow the heuristic to
    stay in Set, which is necessary to get along with the MetaCoq in Prototype.v.
 
@@ -34,22 +39,14 @@ CoInductive InlineHeuristic : Set := {
   update_funDef : fundefs -> InlineHeuristic * InlineHeuristic;
   (* Update inlining decisions when converting a function within a bundle *)
   update_inFun : var -> fun_tag -> list var -> exp -> InlineHeuristic;
-  (* Update and return inlining decision for f on function application *)
-  update_App : var -> fun_tag -> list var -> InlineHeuristic * bool;
-  (* Update and return inlining decision for f on let bound function application *)
-  update_letApp : var -> fun_tag -> list var -> InlineHeuristic * bool }.
-
-Definition fun_map : Set := M.tree (fun_tag * list var * exp).
-
-Definition freshen_exp (e:exp) (cdata : comp_data) : option (exp * comp_data) :=
-  let '(me, (cdata, tt)) := compM.runState (freshen_term ![e] (M.empty _)) tt (cdata, tt) in
-  match me with
-  | compM.Err _ => None
-  | compM.Ret e => Some ([e]!, cdata)
-  end. (* TODO avoid conversions *)
-
-Definition R_misc : Set := fun_map.
-Definition S_misc : Set := InlineHeuristic * comp_data.
+  (* Return inlining decision on function application *)
+  decide_App : var -> fun_tag -> list var -> bool;
+  (* Update heuristic on function application *)
+  update_App : var -> fun_tag -> list var -> InlineHeuristic;
+  (* Return inlining decision on let bound function application *)
+  decide_letApp : var -> fun_tag -> list var -> bool;
+  (* Update heuristic on let bound function application *)
+  update_letApp : var -> fun_tag -> list var -> InlineHeuristic }.
 
 CoFixpoint CombineInlineHeuristic (deci: bool -> bool -> bool) (IH1 IH2 : InlineHeuristic) : InlineHeuristic := {| 
   update_funDef fds :=
@@ -60,14 +57,22 @@ CoFixpoint CombineInlineHeuristic (deci: bool -> bool -> bool) (IH1 IH2 : Inline
     let IH1' := IH1.(update_inFun) f ft xs e in
     let IH2' := IH2.(update_inFun) f ft xs e in
     CombineInlineHeuristic deci IH1' IH2';
+  decide_App f ft ys :=
+    let b1 := IH1.(decide_App) f ft ys in
+    let b2 := IH2.(decide_App) f ft ys in
+    deci b1 b2;
   update_App f ft ys :=
-    let (IH1', b1) := IH1.(update_App) f ft ys in
-    let (IH2', b2) := IH2.(update_App) f ft ys in
-    (CombineInlineHeuristic deci IH1' IH2', deci b1 b2);
+    let IH1' := IH1.(update_App) f ft ys in
+    let IH2' := IH2.(update_App) f ft ys in
+    CombineInlineHeuristic deci IH1' IH2';
+  decide_letApp f ft ys :=
+    let b1 := IH1.(decide_App) f ft ys in
+    let b2 := IH2.(decide_App) f ft ys in
+    deci b1 b2;
   update_letApp f ft ys :=
-    let (IH1', b1) := IH1.(update_App) f ft ys in
-    let (IH2', b2) := IH2.(update_App) f ft ys in
-    (CombineInlineHeuristic deci IH1' IH2', deci b1 b2) |}.
+    let IH1' := IH1.(update_App) f ft ys in
+    let IH2' := IH2.(update_App) f ft ys in
+    CombineInlineHeuristic deci IH1' IH2' |}.
 
 Definition PostUncurryIH : M.t nat -> InlineHeuristic :=
   cofix IH s := {|
@@ -75,13 +80,19 @@ Definition PostUncurryIH : M.t nat -> InlineHeuristic :=
     (* 0 -> Do not inline, 1 -> uncurried function, 2 -> continuation of uncurried function *)
     update_funDef fds := let IH' := IH s in (IH', IH');
     update_inFun f ft xs e := IH s;
+    decide_App f ft ys :=
+      match (M.get ![f] s, ys) with
+      | (Some 1, _::_) => true
+      | (Some 2, _) => true
+      | _ => false
+      end;
     update_App f ft ys :=
       match (M.get ![f] s, ys) with
-      | (Some 1, k::ys') => (IH (M.set ![f] 0 (M.set ![k] 2 s)), true)
-      | (Some 2, _) => (IH s, true)
-      | _ => (IH s, false)
+      | (Some 1, k::ys') => IH (M.set ![f] 0 (M.set ![k] 2 s))
+      | _ => IH s
       end;
-    update_letApp f t ys := (IH s, false) |}.
+    decide_letApp f t ys := false;
+    update_letApp f t ys := IH s |}.
 
 Definition InlineSmallIH (bound : nat) : M.t bool -> InlineHeuristic :=
   cofix IH s := {|
@@ -99,12 +110,18 @@ Definition InlineSmallIH (bound : nat) : M.t bool -> InlineHeuristic :=
       let IH' := IH (upd fds s) in
       (IH', IH');
     update_inFun f ft xs e := IH (M.remove ![f] s);
+    decide_App f ft ys :=
+      match M.get ![f] s with
+      | Some true => true
+      | _ => false
+      end;
     update_App f ft ys :=
       match M.get ![f] s with
-      | Some true => (IH (M.remove ![f] s), true)
-      | _ => (IH s, false)
+      | Some true => IH (M.remove ![f] s)
+      | _ => IH s
       end;
-    update_letApp f ft ys := (IH s, false) |}.
+    decide_letApp f ft ys := false;
+    update_letApp f ft ys := IH s |}.
 
 Open Scope positive.
 
@@ -117,16 +134,18 @@ Fixpoint find_uncurried (fds : fundefs) (s:M.t bool) : M.t bool :=
   | _ => s
   end.
 
-Definition InineUncurried : M.t bool -> InlineHeuristic :=
+Definition InlineUncurried : M.t bool -> InlineHeuristic :=
   cofix IH s := {|
     update_funDef fds := let IH' := IH (find_uncurried fds s) in (IH', IH');
     update_inFun f ft xs e := IH (M.remove ![f] s);
-    update_App f ft ys :=
+    decide_App f ft ys :=
       match M.get ![f] s with
-      | Some true => (IH s, true)
-      | _ => (IH s, false)
+      | Some true => true
+      | _ => false
       end;
-    update_letApp f ft ys := (IH s, false) |}.
+    update_App f ft ys := IH s;
+    decide_letApp f ft ys := false;
+    update_letApp f ft ys := IH s |}.
 
 Fixpoint find_uncurried_pats_anf (fds : fundefs) (s:M.t bool) : M.t bool :=
   match fds with
@@ -149,16 +168,18 @@ Definition InineUncurriedPatsAnf : M.t bool -> InlineHeuristic :=
       let IH' := IH (find_uncurried fds s) in
       (IH', IH');
     update_inFun f ft xs e := IH (M.remove ![f] s);
-    update_App f ft ys :=
+    decide_App f ft ys :=
       match M.get ![f] s with
-      | Some true => (IH s, true)
-      | _ => (IH s, false)
+      | Some true => true
+      | _ => false
       end;
-    update_letApp f ft ys :=
+    update_App f ft ys := IH s;
+    decide_letApp f ft ys :=
       match M.get ![f] s with
-      | Some true => (IH s, true)
-      | _ => (IH s, false)
-      end |}.
+      | Some true => true
+      | _ => false
+      end;
+    update_letApp f ft ys := IH s |}.
 
 Definition InlinedUncurriedMarkedAnf : M.t nat -> InlineHeuristic :=
   cofix IH s := {|
@@ -166,21 +187,732 @@ Definition InlinedUncurriedMarkedAnf : M.t nat -> InlineHeuristic :=
     (* 0 -> Do not inline, 1 -> uncurried function, 2 -> continuation of uncurried function *)
     update_funDef fds := let IH' := IH s in (IH', IH');
     update_inFun f ft xs e := IH s;
+    decide_App f ft ys :=
+      match M.get ![f] s with
+      | Some 1%nat => true
+      | Some 2%nat => true
+      | _ => false
+      end;
     update_App f ft ys :=
       match M.get ![f] s with
-      | Some 1%nat => (IH (M.set ![f] 0%nat s), true)
-      | Some 2%nat => (IH (M.set ![f] 0%nat s), true)
-      | _ => (IH s, false)
+      | Some 1%nat => IH (M.set ![f] 0%nat s)
+      | Some 2%nat => IH (M.set ![f] 0%nat s)
+      | _ => IH s
       end;
-    update_letApp f ft ys :=
+    decide_letApp f ft ys :=
       match M.get ![f] s with
-      | Some 1%nat => (IH s, true)
-      | Some 2%nat => (IH s, true)
-      | _ => (IH s, false)
-      end |}.
+      | Some 1%nat => true
+      | Some 2%nat => true
+      | _ => false
+      end;
+    update_letApp f ft ys := IH s |}.
 
 Definition InlineSmallOrUncurried (bound : nat) (s1 : M.t bool) (s2 : M.t nat) : InlineHeuristic :=
   CombineInlineHeuristic orb (InlineSmallIH bound s1) (PostUncurryIH s2).
+
+(** * Inlining as a relation *)
+
+Definition R_misc : Set := InlineHeuristic.
+Definition S_misc : Set := comp_data.
+
+Definition update_next_var (next : cps.var) (cdata : comp_data) : comp_data := 
+  let '{| next_var := _; nect_ctor_tag := c; next_ind_tag := i; next_fun_tag := f;
+          cenv := e; fenv := fenv; nenv := names; log := log |} := cdata
+  in
+  {| next_var := next; nect_ctor_tag := c;
+     next_ind_tag := i; next_fun_tag := f; cenv := e; fenv := fenv;
+     nenv := names; log := log |}.
+
+Fixpoint find_def (f : var) (fds : fundefs) :=
+  match fds with
+  | Fcons f' ft xs e fds => if Pos.eqb ![f] ![f'] then Some (ft, xs, e) else find_def f fds
+  | Fnil => None
+  end.
+
+(* The function definition f(xs) = e_body (with fun tag ft) is in scope at C⟦e⟧ if... *)
+Definition known_function {A} (f : var) (ft : fun_tag) (xs : list var) (e_body : exp)
+          (C : exp_c A exp_univ_exp) (e : univD A) : Prop :=
+  (* ...f was defined in a bundle encountered earlier... *)
+  (exists D fds E, C = D >:: Efun1 fds >++ E /\ List.In (f, ft, xs, e_body) [fds]!) \/
+  (* ...or f is in a bundle and we are currently inside one of the bundle's definitions... *)
+  (exists D fds1 g gt ys fds2 E,
+    C = D >++ ctx_of_fds fds1 >:: Fcons3 g gt ys fds2 >++ E /\
+    (List.In (f, ft, xs, e_body) fds1 \/ find_def f fds2 = Some (ft, xs, e_body))) \/
+  (* ...or f is in a bundle that we are currently traversing *)
+  (match A return exp_c A exp_univ_exp -> univD A -> Prop with
+   | exp_univ_fundefs => fun C fds2 => exists D fds1,
+     C = D >++ ctx_of_fds fds1 /\
+     (List.In (f, ft, xs, e_body) fds1 \/ find_def f fds2 = Some (ft, xs, e_body))
+   | _ => fun _ _ => False
+   end C e).
+
+Inductive inline_step : exp -> exp -> Prop :=
+(* Update heuristic at each Efun node *)
+| inline_update_Efun :
+  forall (C : frames_t exp_univ_exp exp_univ_exp) fds e IH IH1 IH2,
+  (IH1, IH2) = IH.(update_funDef) fds ->
+  When (fun (r : R_misc) (s : S_misc) => true) ->
+  inline_step
+    (C ⟦ Efun fds e ⟧)
+    (C ⟦ Efun (Local (fun _ => IH1) (Rec fds)) (Local (fun _ => IH2) (Rec e)) ⟧)
+(* Update heuristic at each Fcons node *)
+| inline_update_Fcons :
+  forall (C : frames_t exp_univ_fundefs exp_univ_exp) f ft xs e fds,
+  When (fun (r : R_misc) (s : S_misc) => true) ->
+  inline_step
+    (C ⟦ Fcons f ft xs e fds ⟧)
+    (C ⟦ Fcons f ft xs (Local (fun IH => IH.(update_inFun) f ft xs e) e) (Rec fds) ⟧)
+(* Inlining for CPS *)
+| inline_cps :
+  forall (C : frames_t exp_univ_exp exp_univ_exp) f ft (xs : list var) e e' (ys : list var) lhs next_x,
+  lhs = Eapp f ft ys ->
+  known_function f ft xs e C lhs ->
+  Alpha_conv ![e] ![e'] (id <{ ![xs] ~> ![ys] }>) ->
+  Disjoint _ (bound_var ![e']) (used_vars ![C ⟦ lhs ⟧]) ->
+  fresher_than next_x (used_vars ![C ⟦ lhs ⟧] :|: used e') ->
+  (* Only inline if the inlining heuristic decides to *)
+  When (fun (IH : R_misc) (s : S_misc) => IH.(decide_App) f ft ys) ->
+  inline_step
+    (C ⟦ Eapp f ft ys ⟧)
+    (C ⟦ (* Update inlining heuristic *)
+         Local (fun IH => IH.(update_App) f ft ys)
+         (* Hack: set fresh variable in cdata properly for future passes *)
+         (Modify (update_next_var next_x)
+         (Rec e')) ⟧).
+
+(* Maintain map of known functions while traversing *)
+Definition S_fns {A} (C : exp_c A exp_univ_exp) (e : univD A) : Set := {
+  ρ : M.tree (fun_tag * list var * exp) | 
+  forall f ft xs e_body, M.get f ρ = Some (ft, xs, e_body) ->
+  known_function [f]! ft xs e_body C e }.
+
+(* TODO: move the following lemmas to cps_proto.v *)
+
+Instance exp_Frame_inj : Frame_inj exp_univ.
+Proof. intros A B f x y; destruct f; now inversion 1. Qed.
+
+Require Import Coq.Logic.JMeq.
+Require Import Coq.Logic.Eqdep.
+Ltac inv_ex :=
+  repeat progress match goal with
+  | H : existT ?P ?T _ = existT ?P ?T _ |- _ => apply inj_pairT2 in H
+  end.
+
+(* Inhabited types *)
+
+Class Inhabited A := inhabitant : A.
+
+Instance Inhabited_pos : Inhabited positive := xH.
+Instance Inhabited_var : Inhabited var := mk_var inhabitant.
+Instance Inhabited_fun_tag : Inhabited fun_tag := mk_fun_tag inhabitant.
+Instance Inhabited_ctor_tag : Inhabited ctor_tag := mk_ctor_tag inhabitant.
+Instance Inhabited_prim : Inhabited prim := mk_prim inhabitant.
+Instance Inhabited_N : Inhabited N := N0.
+
+Instance Inhabited_exp : Inhabited exp := Ehalt inhabitant.
+Instance Inhabited_fundefs : Inhabited fundefs := Fnil.
+
+Instance Inhabited_list A : Inhabited (list A) := [].
+Instance Inhabited_prod A B `{Inhabited A} `{Inhabited B} : Inhabited (A * B) := (inhabitant, inhabitant).
+
+Definition univ_inhabitant {A} : univD A :=
+  match A with
+  | exp_univ_prod_ctor_tag_exp => inhabitant
+  | exp_univ_list_prod_ctor_tag_exp => inhabitant
+  | exp_univ_fundefs => inhabitant
+  | exp_univ_exp => inhabitant
+  | exp_univ_var => inhabitant
+  | exp_univ_fun_tag => inhabitant
+  | exp_univ_ctor_tag => inhabitant
+  | exp_univ_prim => inhabitant
+  | exp_univ_N => inhabitant
+  | exp_univ_list_var => inhabitant
+  end.
+
+(* Inhabited types, with assumption that inhabited <> inhabited' *)
+
+Class Inhabited' A := inhabitant' : A.
+
+Instance Inhabited'_pos : Inhabited' positive := xO xH.
+Instance Inhabited'_var : Inhabited' var := mk_var inhabitant'.
+Instance Inhabited'_fun_tag : Inhabited' fun_tag := mk_fun_tag inhabitant'.
+Instance Inhabited'_ctor_tag : Inhabited' ctor_tag := mk_ctor_tag inhabitant'.
+Instance Inhabited'_prim : Inhabited' prim := mk_prim inhabitant'.
+Instance Inhabited'_N : Inhabited' N := Npos inhabitant'.
+
+Instance Inhabited'_list A `{Inhabited' A} : Inhabited' (list A) := [inhabitant'].
+Instance Inhabited'_prod A B `{Inhabited' A} `{Inhabited' B} : Inhabited' (A * B) := (inhabitant', inhabitant').
+
+Instance Inhabited'_exp : Inhabited' exp := Ehalt inhabitant'.
+Instance Inhabited'_fundefs : Inhabited' fundefs := Fcons inhabitant' inhabitant' inhabitant' inhabitant' Fnil.
+
+Lemma frame_ext_eq' {A B A' B'} (f : exp_frame_t A B) (g : exp_frame_t A' B') :
+  A = A' -> B = B' ->
+  (forall x x', JMeq x x' -> JMeq (frameD f x) (frameD g x')) -> JMeq f g.
+Proof.
+  destruct f, g; try congruence; simpl; intros _ _ Hext;
+  pose (Hext1 := Hext inhabitant inhabitant JMeq_refl); clearbody Hext1;
+  pose (Hext2 := Hext inhabitant' inhabitant' JMeq_refl); clearbody Hext2;
+  inversion Hext1; inversion Hext2; inv_ex;
+  repeat match goal with H : _ = _ |- _ => inv H end; constructor.
+Qed.
+
+Corollary frame_ext_eq {A B} (f g : exp_frame_t A B) :
+  (forall x, frameD f x = frameD g x) -> f = g.
+Proof.
+  intros Hext; enough (JMeq f g) by now apply JMeq_eq.
+  apply frame_ext_eq'; auto; intros x x' Hxx'.
+  inversion Hxx'; inv_ex; subst x'.
+  specialize (Hext x); rewrite Hext; now constructor.
+Qed.
+
+Class Sized A := size : A -> nat.
+
+Fixpoint size_pos (n : positive) :=
+  match n with
+  | xI x => S (size_pos x)
+  | xO x => S (size_pos x)
+  | xH => 1%nat
+  end.
+Instance Sized_pos : Sized positive := size_pos.
+
+Instance Sized_var : Sized var := fun '(mk_var x) => S (size x).
+Instance Sized_fun_tag : Sized fun_tag := fun '(mk_fun_tag x) => S (size x).
+Instance Sized_ctor_tag : Sized ctor_tag := fun '(mk_ctor_tag x) => S (size x).
+Instance Sized_prim : Sized prim := fun '(mk_prim x) => S (size x).
+Instance Sized_N : Sized N := fun n => match n with N0 => 1%nat | Npos x => S (size x) end.
+
+Definition size_list {A} (size : A -> nat) : list A -> nat := fold_right (fun x n => S (size x + n)) 1%nat.
+Definition size_prod {A B} (sizeA : A -> nat) (sizeB : B -> nat) : A * B -> nat := fun '(x, y) => S (sizeA x + sizeB y).
+
+Instance Size_list A `{Sized A} : Sized (list A) := size_list size.
+Instance Size_prod A B `{Sized A} `{Sized B} : Sized (A * B) := size_prod size size.
+
+Fixpoint size_exp (e : exp) : nat with size_fundefs (fds : fundefs) : nat.
+Proof.
+- refine (match e with
+  | Econstr x c ys e => S (size x + size c + size ys + size_exp e)
+  | Ecase x ces => S (size x + size_list (size_prod size size_exp) ces)
+  | Eproj x c n y e => S (size x + size c + size n + size y + size_exp e)
+  | Eletapp x f ft ys e => S (size x + size f + size ft + size ys + size_exp e)
+  | Efun fds e => S (size_fundefs fds + size_exp e)
+  | Eapp f ft xs => S (size f + size ft + size xs)
+  | Eprim x p ys e => S (size x + size p + size ys + size_exp e)
+  | Ehalt x => S (size x)
+  end).
+- refine (match fds with
+  | Fcons f ft xs e fds => S (size f + size ft + size xs + size_exp e + size_fundefs fds)
+  | Fnil => 1%nat
+  end).
+Defined.
+
+Instance Sized_exp : Sized exp := size_exp.
+Instance Sized_fundefs : Sized fundefs := size_fundefs.
+
+Definition univ_size {A} : univD A -> nat :=
+  match A with
+  | exp_univ_prod_ctor_tag_exp => size
+  | exp_univ_list_prod_ctor_tag_exp => size
+  | exp_univ_fundefs => size
+  | exp_univ_exp => size
+  | exp_univ_var => size
+  | exp_univ_fun_tag => size
+  | exp_univ_ctor_tag => size
+  | exp_univ_prim => size
+  | exp_univ_N => size
+  | exp_univ_list_var => size
+  end.
+
+Lemma frame_size_gt {A B} (f : exp_frame_t A B) (x : univD A) :
+  (univ_size (frameD f x) > univ_size x)%nat.
+Proof.
+  destruct f; cbn;
+  try change (size_exp x) with (size x); cbn;
+  try change (size_fundefs x) with (size x); cbn;
+  try change (size_list (size_prod size size) x) with (size x); cbn;
+  lia.
+Qed.
+
+Fixpoint exp_c_size_ge {A B} (C : exp_c A B) (x : univD A) {struct C} :
+  (univ_size (C ⟦ x ⟧) >= univ_size x)%nat.
+Proof.
+  destruct C as [|A AB B f C]; simpl; [lia|].
+  assert (univ_size (C ⟦ exp_frameD A AB f x ⟧) >= univ_size (frameD f x))%nat by apply exp_c_size_ge.
+  assert (univ_size (frameD f x) > univ_size x)%nat by apply frame_size_gt.
+  lia.
+Qed.
+
+Definition exp_c_size_eq {A B} (C : exp_c A B) (x : univD A) :
+  univ_size (C ⟦ x ⟧) = univ_size x -> JMeq C (<[]> : exp_c A A).
+Proof.
+  destruct C as [|A AB B f C]; simpl; [constructor|intros HC].
+  assert (univ_size (C ⟦ exp_frameD A AB f x ⟧) >= univ_size (exp_frameD A AB f x))%nat
+   by apply exp_c_size_ge.
+  assert (univ_size (exp_frameD A AB f x) > univ_size x)%nat by apply frame_size_gt.
+  lia.
+Qed.
+
+Lemma exp_ext_nil {A B} (C : exp_c A B) : A = B -> (forall x, JMeq x (C ⟦ x ⟧)) -> JMeq C (<[]> : exp_c A A).
+Proof.
+  destruct C as [|A AB B f C]; [constructor|simpl].
+  intros HeqB Hext; subst; specialize (Hext univ_inhabitant).
+  inversion Hext; inv_ex.
+  apply f_equal with (f := univ_size) in H.
+  match type of Hext with
+  | JMeq _ (?C ⟦ ?f ⟧) =>
+    match f with
+    | exp_frameD _ _ _ ?x =>
+      assert (univ_size (C ⟦ f ⟧) >= univ_size f)%nat by apply exp_c_size_ge;
+      assert (univ_size f > univ_size x)%nat by apply frame_size_gt;
+      lia
+    end
+  end.
+Qed.
+
+Corollary exp_ext_nil' {A B} (C : exp_c A B) : A = B -> (forall x, JMeq x (C ⟦ x ⟧)) -> JMeq C (<[]> : exp_c B B).
+Proof. intros; subst; now apply exp_ext_nil. Qed.
+
+Lemma exp_c_ext_eq' {A B A'} (C : exp_c A B) (D : exp_c A' B) :
+  A = A' -> (forall x x', JMeq x x' -> C ⟦ x ⟧ = D ⟦ x' ⟧) -> JMeq C D.
+Proof.
+  remember (frames_len C + frames_len D)%nat as n eqn:Heqn.
+  revert A B A' C D Heqn; induction n as [n IHn] using lt_wf_ind.
+  intros A B A' C D Heqn Heq Hext.
+  destruct (frames_split C) as [[AB [g [C' HC]]] | HClen0];
+  destruct (frames_split D) as [[AB' [g' [D' HD]]] | HDlen0].
+  - admit.
+  - admit.
+  - admit.
+  - destruct C, D; simpl in HClen0, HDlen0; try congruence; constructor.
+Admitted.
+(*
+  destruct C, D.
+  - constructor.
+  - intros Heq Hext; apply JMeq_sym; apply exp_ext_nil'; [congruence|].
+    subst; intros x; specialize (Hext x x JMeq_refl); simpl in *; rewrite <- Hext; constructor.
+  - intros Heq Hext; subst; apply exp_ext_nil; [congruence|].
+    intros x; specialize (Hext x x JMeq_refl); simpl in *; rewrite Hext; constructor.
+  - 
+    intros ? Hwat; subst; simpl in *.
+    clear - Hwat.
+  destruct f, g; try congruence; simpl; intros _ _ Hext;
+  pose (Hext1 := Hext inhabitant inhabitant JMeq_refl); clearbody Hext1;
+  pose (Hext2 := Hext inhabitant' inhabitant' JMeq_refl); clearbody Hext2;
+  inversion Hext1; inversion Hext2; inv_ex;
+  repeat match goal with H : _ = _ |- _ => inv H end; constructor.
+Qed. *)
+
+(*
+Lemma ctx_cons_inj U V1 V2 W
+      (f : exp_frame_t U V1) (C : exp_c V1 W)
+      (g : exp_frame_t U V2) (D : exp_c V2 W) :
+  JMeq (C >:: f) (D >:: g) -> V1 = V2 /\ JMeq f g /\ JMeq C D.
+Proof.
+  destruct f, g.
+  inversion 1; inv_ex;
+  try lazymatch goal with H : _ >:: _ = _ >:: _ |- _ => inversion H end;
+  inv_ex; subst; repeat split; try constructor.
+  inversion 1.
+  inv_ex. *)
+
+Definition uframe_t {U : Set} `{H : Frame U} := {A & {B & @frame_t U H A B}}.
+Definition uframes_t {U : Set} `{H : Frame U} := list (@uframe_t U H).
+
+Fixpoint well_typed {U : Set} `{H : Frame U} (A B : U) (fs : @uframes_t U H) : Prop.
+Proof.
+  destruct fs as [|f fs]; [exact (A = B)|].
+  destruct f as [A' [AB f]].
+  exact (A = A' /\ well_typed U H AB B fs).
+Defined.
+
+Fixpoint untype {U : Set} `{H : Frame U} {A B : U} (fs : @frames_t U H A B) : @uframes_t U H.
+Proof.
+  destruct fs as [|A AB B f fs]; [exact []|refine (_ :: _)].
+  - do 2 eexists; exact f.
+  - eapply untype; exact fs.
+Defined.
+
+Fixpoint untype_well_typed {U : Set} `{H : Frame U} {A B : U} (fs : @frames_t U H A B) :
+  well_typed A B (untype fs).
+Proof.
+  destruct fs as [|A AB B f fs]; [reflexivity|simpl].
+  split; [reflexivity|now apply untype_well_typed].
+Defined.
+
+Fixpoint retype {U : Set} `{H : Frame U} (A B : U) (fs : @uframes_t U H)
+         (Hty : well_typed A B fs) {struct fs} : 
+  @frames_t U H A B.
+Proof.
+  destruct fs as [|[A' [AB f]] fs]; simpl in Hty.
+  - subst; exact <[]>.
+  - destruct Hty; subst.
+    refine (_ >:: f).
+    now eapply retype.
+Defined.
+
+Definition frames_sig_t {U : Set} `{H : Frame U} A B := {fs : @uframes_t U H | well_typed A B fs}.
+
+Definition ty_split {U : Set} `{H : Frame U} {A B : U} (fs : @frames_t U H A B) : @frames_sig_t U H A B.
+Proof. exists (untype fs); now apply untype_well_typed. Defined.
+
+Definition ty_merge {U : Set} `{H : Frame U} {A B : U} : @frames_sig_t U H A B -> @frames_t U H A B.
+Proof. intros [fs Hfs]; now eapply retype. Defined.
+
+Fixpoint t_sig_t {U : Set} `{H : Frame U} {A B : U} (fs : @frames_t U H A B) :
+  ty_merge (ty_split fs) = fs.
+Proof.
+  destruct fs as [|A AB B f fs]; [reflexivity|simpl].
+  unfold eq_rec_r, eq_rec, eq_rect, eq_sym; f_equal.
+  rewrite <- t_sig_t; reflexivity.
+Qed.
+
+Fixpoint sig_t_sig' {U : Set} `{H : Frame U} {A B : U} (fs : @uframes_t U H)
+         (Hty : @well_typed U H A B fs) {struct fs} :
+  ty_split (ty_merge (exist _ fs Hty)) = (exist _ fs Hty).
+Proof.
+  destruct fs as [|[A' [AB' f]] fs]; simpl in Hty.
+  - subst; reflexivity.
+  - destruct Hty as [? Hwt]; subst; cbn; unfold ty_split; cbn.
+    apply ProofIrrelevance.ProofIrrelevanceTheory.subset_eq_compat.
+    specialize (sig_t_sig' U H _ _ fs Hwt).
+    apply (@f_equal _ _ (@proj1_sig _ _)) in sig_t_sig'; cbn in sig_t_sig'.
+    now rewrite sig_t_sig'.
+Defined.
+
+Definition sig_t_sig {U : Set} `{H : Frame U} {A B : U} (fs : @frames_sig_t U H A B) :
+  ty_split (ty_merge fs) = fs.
+Proof. destruct fs as [fs Hfs]; apply sig_t_sig'. Defined.
+
+Instance Iso_frames {U : Set} `{H : Frame U} {A B : U} : Iso (@frames_t U H A B) (@frames_sig_t U H A B) := {
+  isoAofB := ty_merge;
+  isoBofA := ty_split;
+  isoABA := t_sig_t;
+  isoBAB := sig_t_sig }.
+
+(* If not entering or exiting a function bundle, the set of known functions remains the same *)
+
+(* Inductive frames_eq {U : Set} `{Frame U} : forall {A B A' B' : U}, frames_t A B -> frames_t A' B' -> Prop := *)
+(* | frames_eq_nil : forall A A', A = A' -> frames_eq (<[]> : frames_t A A) (<[]> : frames_t A' A'). *)
+(* | frames_eq_cons : forall A AB B A' AB' B', A = A' -> frames_eq (<[]> : frames_t A A) (<[]> : frames_t A' A'). *)
+
+Fixpoint frames_eq {U : Set} `{Frame U} {A B A' B' : U} (fs : frames_t A B) (gs : frames_t A' B') : Prop.
+Proof.
+  destruct fs as [|A AB B f fs]; destruct gs as [|A' AB' B' g gs].
+  - exact (A = A0).
+  - exact False.
+  - exact False.
+  - refine (exists (HA : A = A') (HAB : AB = AB'), _).
+    subst; refine (f = g /\ _).
+    eapply frames_eq; [exact fs|exact gs].
+Defined.
+
+(* Infix "~=" := Feq (at level 80, no associativity). *)
+
+Definition frames_split' {U : Set} {F : U -> U -> Set} {A B} (fs : frames_t' F A B) :
+  (exists AB (g : F A AB) (gs : frames_t' F AB B), fs = gs >:: g) \/ (frames_len fs = O).
+Proof. destruct fs as [| A' AB B' f fs]; [now right|left; now do 3 eexists]. Qed.
+
+Fixpoint eq_frames_eq {U : Set} `{Frame U} {A B : U}
+      (fs gs : frames_t A B) :
+  fs = gs -> frames_eq fs gs.
+Proof.
+  destruct fs; destruct (frames_split' gs) as [[AA [g [gs' Hgs]]]|Hglen].
+  - subst gs; now inversion 1.
+  - intros Hnil; subst; reflexivity.
+  - subst gs; inversion 1; subst; inv_ex; simpl; exists eq_refl, eq_refl; cbn.
+    split; [auto|now apply eq_frames_eq].
+  - destruct gs; [inversion 1|inversion Hglen].
+Qed.
+
+Fixpoint frames_eq_eq {U : Set} `{Frame U} {A B : U}
+      {fs gs : frames_t A B} :
+  frames_eq fs gs -> fs = gs.
+Proof.
+  destruct fs; destruct (frames_split' gs) as [[AB [g [gs' Hgs]]]|Hglen].
+  - subst gs; inversion 1.
+  - admit.
+  - subst gs; simpl.
+    unfold eq_rect_r, eq_rect, eq_sym.
+    intros [HA [HAB Heqs]].
+Admitted.
+
+Lemma eq_JMeq {A} {x y : A} (H : x = y) : JMeq x y. Proof. subst; constructor. Qed.
+
+Lemma known_nonbundle_dn {A B} (C : exp_c B exp_univ_exp) (fr : exp_frame_t A B)
+      (e : univD A) f ft xs e_body :
+  A <> exp_univ_fundefs -> B <> exp_univ_fundefs ->
+  known_function f ft xs e_body C (frameD fr e) ->
+  known_function f ft xs e_body (C >:: fr) e.
+Proof.
+  destruct fr; try congruence; intros _ _ Hknown;
+  solve [
+    destruct Hknown as [[D [fds [E [HC Hfxs]]]] | [[D [fds1 [g [gt [ys [fds2 [E [HC Hfxs]]]]]]]] | []]];
+    [left|right; left]; subst C; repeat eexists;
+    try match goal with |- _ /\ _ => split end; try match goal with
+    | |- context [?fs >++ ?gs >:: ?g] => change (fs >++ gs >:: g) with (fs >++ (gs >:: g))
+    end; try reflexivity; try assumption].
+Qed.
+
+Lemma known_nonbundle_up {A B} (C : exp_c B exp_univ_exp) (fr : exp_frame_t A B)
+      (e : univD A) f ft xs e_body :
+  A <> exp_univ_fundefs -> B <> exp_univ_fundefs ->
+  known_function f ft xs e_body (C >:: fr) e ->
+  known_function f ft xs e_body C (frameD fr e).
+Proof.
+  destruct fr; try congruence; intros _ _ Hknown.
+    destruct Hknown as [[D [fds [E [HC Hfxs]]]] | [[D [fds1 [g [gt [ys [fds2 [E [HC Hfxs]]]]]]]] | []]];
+    [left|right; left].
+    apply eq_frames_eq in HC.
+    destruct (frames_split' E) as [[AB [Ef [E' HE]]] | HElen]; [subst E|].
+    simpl in HC.
+    apply frames_eq_eq in HC.
+    inversion HC; inv_ex.
+    inversion HC.
+    inversion HC.
+    apply inj_pairT2 in H0.
+    inversion H0.
+    apply inj_pairT2 in H2.
+    Check inj_pairT2.
+    SearchAbout existT.
+    subst E.
+    destruct E.
+
+    subst C; repeat eexists;
+    try match goal with |- _ /\ _ => split end; try match goal with
+    | |- context [?fs >++ ?gs >:: ?g] => change (fs >++ gs >:: g) with (fs >++ (gs >:: g))
+    end; try reflexivity; try assumption.
+Defined.
+
+
+(* The function definition f(xs) = e_body (with fun tag ft) is in scope at C⟦e⟧ if... *)
+Definition known_function {A} (f : var) (ft : fun_tag) (xs : list var) (e_body : exp)
+          (C : exp_c A exp_univ_exp) (e : univD A) : Prop :=
+  (* ...f was defined in a bundle encountered earlier... *)
+  (exists D fds E, C = D >:: Efun1 fds >++ E /\ List.In (f, ft, xs, e_body) [fds]!) \/
+  (* ...or f is in a bundle and we are currently inside one of the bundle's definitions... *)
+  (exists D fds1 g gt ys fds2 E,
+    C = D >++ ctx_of_fds fds1 >:: Fcons3 g gt ys fds2 >++ E /\
+    (List.In (f, ft, xs, e_body) fds1 \/ find_def f fds2 = Some (ft, xs, e_body))) \/
+  (* ...or f is in a bundle that we are currently traversing *)
+  (match A return exp_c A exp_univ_exp -> univD A -> Prop with
+   | exp_univ_fundefs => fun C fds2 => exists D fds1,
+     C = D >++ ctx_of_fds fds1 /\
+     (List.In (f, ft, xs, e_body) fds1 \/ find_def f fds2 = Some (ft, xs, e_body))
+   | _ => fun _ _ => False
+   end C e).
+
+Instance Preserves_S : Preserves_S _ exp_univ_exp (@S_fns).
+Proof.
+  constructor.
+  (* Moving upwards *)
+  - admit.
+  (* Moving downwards *)
+  - intros A B C f e [ρ Hρ].
+    destruct f; lazymatch goal with
+    (* There are only a few cases that we care about: *)
+    | |- S_fns (C >:: Efun0 ?fds) ?e => idtac
+    | |- S_fns (C >:: Efun1 ?e) ?fds => idtac
+    | |- S_fns (C >:: Fcons3 ?f ?ft ?xs ?fds) ?e => idtac
+    | |- S_fns (C >:: Fcons4 ?f ?ft ?xs ?e) ?fds => idtac
+    (* For all the others, the map should remain unchanged *)
+    | _ =>
+      exists ρ; intros f' ft' xs' e' Hftxse';
+      specialize (Hρ f' ft' xs' e' Hftxse')
+    end.
+  (* Before entering the body of a function f, need to delete ρ(f) and add fds *)
+  - rename v into f, f into ft, l into xs, f0 into fds; destruct f as [f].
+    exists (M.remove f ρ); intros g gt ys e Hget.
+    destruct (Pos.eq_dec g f) as [Hgf|Hgf]; [subst; now rewrite M.grs in Hget|].
+    rewrite M.gro in Hget by auto; now apply known_function_cons.
+  (* When moving on from one function f(xs) = e body, need to update ρ(f) *)
+  - rename v into f, f into ft, l into xs; destruct f as [f].
+    exists (M.set f (ft, xs, e) ρ); intros g gt ys eg Hget.
+    destruct (Pos.eq_dec g f) as [Hgf|Hgf];
+      [subst f|rewrite M.gso in Hget by auto; now apply known_function_cons].
+    rewrite M.gss in Hget; inv Hget.
+    unfold known_function.
+    + admit.
+    + rewrite M.gso in Hget by auto; now apply known_function_cons.
+  (* It only remains to show that the extended map satisfies the invariant *)
+  intros f' ft' xs' e' Hget.
+  destruct (Pos.eq_dec f0 f').
+  - subst; rewrite M.gss in Hget; inv Hget; right; left.
+Abort.
+
+(*
+Lemma known_function_cons {A B} f ft xs e_body C (fr : exp_frame_t A B) (e : univD A) :
+  known_function f ft xs e_body C (frameD fr e) ->
+  known_function f ft xs e_body (C >:: fr) e.
+Proof.
+  intros Hknown; destruct fr; solve [
+    destruct Hknown as [[D [fds [E [HC Hfxs]]]] | [D [fds1 [g [gt [ys [fds2 [E [HC Hfxs]]]]]]]]];
+    [left|right]; subst C; repeat eexists;
+    try match goal with |- _ /\ _ => split end; try match goal with
+    | |- context [?fs >++ ?gs >:: ?g] => change (fs >++ gs >:: g) with (fs >++ (gs >:: g))
+    end; try reflexivity; try assumption].
+Qed.
+*)
+
+(*
+Fixpoint add_fundefs (fds:fundefs) ρ :=
+  match fds with
+  | Fnil => ρ
+  | Fcons f t xs e fds => M.set ![f] (t, xs, e) (add_fundefs fds ρ)
+  end.
+*)
+
+Definition r_map : Set := M.tree cps.var.
+
+Fixpoint fun_names (fds : fundefs) : list var :=
+  match fds with
+  | Fnil => []
+  | Fcons f _ _ _ fds => f :: fun_names fds
+  end.
+
+Fixpoint freshen_term (next : positive) (σ : r_map) (e : exp) {struct e} : positive * exp
+with freshen_fun (next : positive) (σ : r_map) (fds : fundefs) {struct fds} : positive * fundefs.
+Proof.
+- refine (
+  match e with
+  | Econstr x c ys e =>
+    let '(next, x') := gensym next in
+    let ys := [apply_r_list σ ![ys]]! in
+    let '(next, e) := freshen_term next (M.set ![x] ![x'] σ) e in
+    (next, Econstr x' c ys e)
+  | Ecase x ces =>
+    let fix freshen_ces next ces {struct ces} :=
+      match ces with
+      | [] => (next, [])
+      | (c, e) :: ces =>
+        let '(next, e) := freshen_term next σ e in
+        let '(next, ces) := freshen_ces next ces in
+        (next, (c, e) :: ces)
+      end
+    in
+    let x := [apply_r σ ![x]]! in
+    let '(next, ces) := freshen_ces next ces in
+    (next, Ecase x ces)
+  | Eproj x c n y e =>
+    let '(next, x') := gensym next in
+    let y := [apply_r σ ![y]]! in
+    let '(next, e) := freshen_term next (M.set ![x] ![x'] σ) e in
+    (next, Eproj x' c n y e)
+  | Eletapp x f ft ys e =>
+    let '(next, x') := gensym next in
+    let f := [apply_r σ ![f]]! in
+    let ys := [apply_r_list σ ![ys]]! in
+    let '(next, e) := freshen_term next (M.set ![x] ![x'] σ) e in
+    (next, Eletapp x' f ft ys e)
+  | Efun fds e =>
+    let fs := fun_names fds in
+    let '(next, fs') := gensyms next fs in
+    match set_lists ![fs] ![fs'] σ with
+    | Some σ =>
+      let '(next, fds) := freshen_fun next σ fds in
+      let '(next, e) := freshen_term next σ e in
+      (next, Efun fds e)
+    | None => (* unreachable *) (next, Efun Fnil e)
+    end
+  | Eapp f ft xs =>
+    let f := [apply_r σ ![f]]! in
+    let xs := [apply_r_list σ ![xs]]! in
+    (next, Eapp f ft xs)
+  | Eprim x p ys e =>
+    let '(next, x') := gensym next in
+    let ys := [apply_r_list σ ![ys]]! in 
+    let '(next, e) := freshen_term next (M.set ![x] ![x'] σ) e in
+    (next, Eprim x' p ys e)
+  | Ehalt x =>
+    let x := [apply_r σ ![x]]! in
+    (next, Ehalt x)
+  end).
+- refine (
+  match fds with
+  | Fcons f ft xs e fds =>
+    let f := [apply_r σ ![f]]! in
+    let '(next, xs') := gensyms next xs in
+    match set_lists ![xs] ![xs'] σ with
+    | Some σ =>
+      let '(next, e) := freshen_term next σ e in
+      let '(next, fds) := freshen_fun next σ fds in
+      (next, Fcons f ft xs' e fds)
+    | None => (* unreachable *) (next, Fnil)
+    end
+  | Fnil => (next, Fnil)
+  end).
+Defined.
+
+Fixpoint freshen_term_spec e {struct e} :
+  forall S next σ next' e',
+  injective_subdomain (occurs_free ![e]) (apply_r σ) ->
+  fresher_than next S ->
+  (next', e') = freshen_term next σ e ->
+  Alpha_conv ![e] ![e'] (apply_r σ) /\
+  Disjoint _ (bound_var ![e']) S /\
+  fresher_than next' (S :|: used_vars ![e'])
+with freshen_fun_spec fds {struct fds} :
+  forall S next σ next' fds',
+  injective_subdomain (occurs_free_fundefs ![fds]) (apply_r σ) ->
+  fresher_than next S ->
+  (next', fds') = freshen_fun next σ fds ->
+  Alpha_conv_fundefs ![fds] ![fds'] (apply_r σ) /\
+  Disjoint _ (bound_var_fundefs ![fds']) S /\
+  fresher_than next' (S :|: used_vars_fundefs ![fds']).
+Proof.
+  - destruct e; intros S next σ next' e'; unbox_newtypes; simpl;
+    repeat match goal with
+    | |- context [let '(_, _) := ?f ?e in _] =>
+      let next := fresh "next" in
+      let e' := fresh "e" in
+      let Hfreshen := fresh "Hfreshen" in
+      destruct (f e) as [next e'] eqn:Hfreshen; symmetry in Hfreshen
+    end.
+Admitted.
+
+(*
+Definition rename' {A} (σ : r_map) : univD A -> univD A :=
+  match A with
+  | exp_univ_prod_ctor_tag_exp => fun '(c, e) => (c, [rename_all σ ![e]]!)
+  | exp_univ_list_prod_ctor_tag_exp => fun ces => map (fun '(c, e) => (c, [rename_all σ ![e]]!)) ces
+  | exp_univ_fundefs => fun fds => [rename_all_fun σ ![fds]]!
+  | exp_univ_exp => fun e => [rename_all σ ![e]]!
+  | exp_univ_var => fun x => [apply_r σ ![x]]!
+  | exp_univ_fun_tag => fun ft => ft
+  | exp_univ_ctor_tag => fun c => c
+  | exp_univ_prim => fun p => p
+  | exp_univ_N => fun n => n
+  | exp_univ_list_var => fun xs => [apply_r_list σ ![xs]]!
+  end.
+*)
+
+(*
+Definition range {A B} (f : A -> option B) : Ensemble B :=
+  fun y => exists x, f x = Some y.
+Definition delay_t {A} (e : univD A) : Set := {
+  σ : r_map |
+  Disjoint _ (range (fun x => M.get x σ)) (used e) /\
+  Disjoint _ (domain (fun x => M.get x σ)) (used e) }.
+Instance Delayed_delay_t : Delayed (@delay_t).
+Proof.
+  unshelve econstructor; [exact @run_delay_t|..].
+  - intros A e; exists (M.empty _).
+    assert (Hdom : domain (fun x => M.get x (M.empty cps.var)) <--> Empty_set _). {
+      split; unfold domain; [intros x Hx; unfold Ensembles.In in Hx|inversion 1].
+      destruct Hx as [y Hy]; now rewrite M.gempty in Hy. }
+    assert (Hran : range (fun x => M.get x (M.empty cps.var)) <--> Empty_set _). {
+      split; unfold codomain; [intros y Hy; unfold Ensembles.In in Hy|inversion 1].
+      destruct Hy as [x Hx]; unfold apply_r in Hx; now rewrite M.gempty in Hx. }
+    rewrite Hdom, Hran; eauto with Ensembles_DB.
+  - destruct A; intros e; simpl in *;
+      try match goal with |- (let '(_, _) := ?rhs in _) = _ => destruct rhs end;
+      try match goal with |- map _ _ = _ => apply MCList.map_id_f; intros [c' e'] end;
+      repeat (rewrite apply_r_empty || rewrite apply_r_list_empty);
+      try rewrite <- (proj1 rename_all_empty); try rewrite <- (proj2 rename_all_empty);
+      unbox_newtypes; normalize_roundtrips; try reflexivity.
+Defined.
+Definition run_delay_t {A} (e : univD A) (d : delay_t e) : univD A := rename' (proj1_sig d) e.
+
+*)
 
 Section Beta.
 
