theories/L6_PCPS/toplevel.v
@@ -3,8 +3,8 @@ Require Import Common.compM.
 From CertiCoq Require Import L6.cps_proto L6.proto_util.
 From CertiCoq Require Import
      L6.cps L6.cps_util L6.state L6.eval L6.shrink_cps L6.inline.
-(* From CertiCoq Require Import L6.uncurry. *)
-From CertiCoq Require Import L6.uncurry_proto.
+From CertiCoq Require Import L6.uncurry.
+(* From CertiCoq Require Import L6.uncurry_proto. *)
 From CertiCoq Require Import L6.L4_to_L6_anf.
 From CertiCoq Require Import L6.L5_to_L6.
 From CertiCoq Require Import L6.closure_conversion L6.hoisting L6.dead_param_elim L6.lambda_lifting.
@@ -121,38 +121,44 @@ Definition L6_pipeline  (opt cps : bool) (args : nat) (no_push : nat) (t : L6_Fu
   in
   let res : error (exp * comp_data):=
       (* uncurring *)
-      (* let '(e_err1, s, c_data) := uncurry_fuel cps 100 (shrink_cps.shrink_top e0) c_data in *)
-      let '(e_pure, s, c_data) := uncurry_top cps 100 c_data [shrink_cps.shrink_top e0]! in
-      let e_err1 := compM.Ret ![e_pure] in
-      (* inlining *)
-      e1 <- e_err1 ;;
-      let (e_err2, c_data) := if cps then inline_uncurry e1 s 10 10 c_data
-                             else inline_uncurry_marked_anf e1 s 10 10 c_data in
-      e2 <- e_err2 ;;
-      (* Shrink reduction *)
-      let e3 := shrink_cps.shrink_top e2 in
-      (* lambda lifting *)
-      let (e_rr4, c_data) := if opt then lambda_lift e3 args no_push c_data else (compM.Ret e3, c_data) in
-      e4 <- e_rr4 ;;
-      (* Shrink reduction *)
-      let e5 := shrink_cps.shrink_top e4 in
-      (* Closure conversion *)
-      let (e_err5, c_data) := closure_conversion.closure_conversion_hoist bogus_closure_tag (* bogus_cloind_tag *) e5 c_data in
-      let '(mkCompData next ctag itag ftag cenv fenv names log) := c_data in
-      e5 <- e_err5 ;;
-      let c_data :=
-          let next_var := ((identifiers.max_var e5 1) + 1)%positive in (* ΧΧΧ check why this is needed *)
-          pack_data next_var ctag itag ftag (add_closure_tag bogus_closure_tag bogus_cloind_tag cenv) fenv (add_binders_exp names e5) log
-      in
-      (* Shrink reduction *)
-      let e6 := shrink_cps.shrink_top e5 in
-      (* Dead parameter elimination *)
-      let (e_err7, c_data) := dead_param_elim.eliminate e6 c_data in
-      (* e7 <- e_err7 ;; *)
-      let e7 := e6 in
-      (* Shrink reduction *)
-      let e8 := shrink_cps.shrink_top e7 in
-      ret (e8, c_data)
+      (* let '(e_pure, s, c_data) := uncurry_top cps 100 c_data [shrink_cps.shrink_top e0]! in *)
+      (* let e_err1 := compM.Ret ![e_pure] in *)
+      let f x := x in
+      let x := f false in
+      if negb (negb x) then (
+        let '(e_err1, s, c_data) := uncurry_fuel cps 100 (shrink_cps.shrink_top e0) c_data in
+        (* inlining *)
+        e1 <- e_err1 ;;
+        let (e_err2, c_data) := if cps then inline_uncurry e1 s 10 10 c_data
+                               else inline_uncurry_marked_anf e1 s 10 10 c_data in
+        e2 <- e_err2 ;;
+        (* Shrink reduction *)
+        let e3 := shrink_cps.shrink_top e2 in
+        (* lambda lifting *)
+        let (e_rr4, c_data) := if opt then lambda_lift e3 args no_push c_data else (compM.Ret e3, c_data) in
+        e4 <- e_rr4 ;;
+        (* Shrink reduction *)
+        let e5 := shrink_cps.shrink_top e4 in
+        (* Closure conversion *)
+        let (e_err5, c_data) := closure_conversion.closure_conversion_hoist bogus_closure_tag (* bogus_cloind_tag *) e5 c_data in
+        let '(mkCompData next ctag itag ftag cenv fenv names log) := c_data in
+        e5 <- e_err5 ;;
+        let c_data :=
+            let next_var := ((identifiers.max_var e5 1) + 1)%positive in (* ΧΧΧ check why this is needed *)
+            pack_data next_var ctag itag ftag (add_closure_tag bogus_closure_tag bogus_cloind_tag cenv) fenv (add_binders_exp names e5) log
+        in
+        (* Shrink reduction *)
+        let e6 := shrink_cps.shrink_top e5 in
+        (* Dead parameter elimination *)
+        let (e_err7, c_data) := dead_param_elim.eliminate e6 c_data in
+        (* e7 <- e_err7 ;; *)
+        let e7 := e6 in
+        (* Shrink reduction *)
+        let e8 := shrink_cps.shrink_top e7 in
+        ret (e8, c_data)
+      ) else (
+        ret ((* shrink_cps.shrink_top *)e0, c_data)
+      )
   in
   match res with
   | compM.Err s =>
